simulation proof on big step semantics

Simu/Cor.v
@@ -1,9 +1,20 @@
-Require Import CommonCor.
-Require Import Sem.
+Require cfrontend.ClightBigstep.
+Require cfrontend.Clight.
+Require Export lib.Integers.
+
+Require Export Rustre.Common.
+Require Export Rustre.RMemory.
+
+Require Export Syn Sem Tra.
+
+Require Export Program.Tactics.
+Require Export List.
+Export List.ListNotations.
+Open Scope list_scope.
 
 (* SIMULATION *)
 
-Section SIMU.
+Section PRESERVATION.
 
   Variable main_node : ident.
   Variable prog: program.
@@ -14,104 +25,537 @@ Section SIMU.
   (* Let ge := globalenv prog. *)
   Let tge := Clight.globalenv tprog.
   
-  Hypothesis TRANSL: translate prog main_node = Errors.OK tprog.
+  Hypothesis TRANSL: translate prog main_node = Errors.OK tprog.    
   (* Hypothesis WF: well_formed prog. *)
   Hypothesis MAINNODE: find_class main_node prog = Some (c_main, cls_main).
 
-     
-  Inductive match_states: state -> Clight.state -> Prop :=
-    intro_state: forall me ve s k e le m,
-      compat_venv c_main ve e m ->
-      compat_menv main_node tprog c_main me e m ->
-      well_formed_stmt c_main s ->
-      compat_stmt main_node tprog me ve e m s ->
-      state_context (me, ve, s) k e le m ->
-      mem_sep main_node c_main e m ->
-      self_sep main_node e m ->
-      fields_sep tprog m ->
-      nodup_env e ->
-      nodup_vars c_main ->
-      nodup_mems c_main ->
-      match_states
-        (me, ve, s)
-        (Clight.State (main_fun main_node c_main) (translate_stmt main_node s) k e le m)
-
-  with state_context: state -> Clight.cont -> Clight.env -> Clight.temp_env -> Memory.Mem.mem -> Prop :=
-       | ctxt_assign: forall me ve x e k env le m,
-           state_context (me, ve, Assign x e) k env le m
-       | ctxt_stassign: forall me ve x e k env le m,
-           state_context (me, ve, AssignSt x e) k env le m
-       | ctxt_ifte: forall me ve e v b s1 s2 k env le m,
-           exp_eval me ve e v ->
-           Cop.bool_val v (typeof e) m = Some b ->
-           match_states
-             (me, ve, if b then s1 else s2)
-             (Clight.State (main_fun main_node c_main)
-                           (translate_stmt main_node (if b then s1 else s2)) k env le m) ->
-           state_context (me, ve, Ifte e s1 s2) k env le m
-       | ctxt_comp: forall me1 ve1 s1 me2 ve2 s2 me3 ve3 k e le m m' m'',
-           match_states
-             (me1, ve1, s1)
-             (Clight.State (main_fun main_node c_main)
-                           (translate_stmt main_node s1)
-                           (Clight.Kseq (translate_stmt main_node s2) k) e le m) ->
-           stmt_eval (me1, ve1, s1) (me2, ve2, Skip) ->
-           match_states
-             (me2, ve2, Skip)
-             (Clight.State (main_fun main_node c_main)
-                           (translate_stmt main_node Skip)
-                           (Clight.Kseq (translate_stmt main_node s2) k) e le m') ->
-           match_states
-             (me2, ve2, s2)
-             (Clight.State (main_fun main_node c_main) (translate_stmt main_node s2) k e le m') ->
-           stmt_eval (me2, ve2, s2) (me3, ve3, Skip) ->
-           match_states
-             (me3, ve3, Skip)
-             (Clight.State (main_fun main_node c_main) (translate_stmt main_node Skip) k e le m'') ->
-           state_context (me1, ve1, Comp s1 s2) k e le m
-       | ctxt_skip_comp: forall me ve s me' ve' k e le m m',
-          match_states
-             (me, ve, s)
-             (Clight.State (main_fun main_node c_main) (translate_stmt main_node s) k e le m) ->
-          stmt_eval (me, ve, s) (me', ve', Skip) ->
-          match_states
-             (me', ve', Skip)
-             (Clight.State (main_fun main_node c_main) (translate_stmt main_node Skip) k e le m') ->
-          state_context (me, ve, Comp Skip s) k e le m
-       | ctxt_skip: forall me ve k e le m,
-           state_context (me, ve, Skip) k e le m.
-  
-  Hint Resolve expr_eval_simu Clight.assign_loc_value sem_cast_same.
-  Hint Constructors compat_stmt state_context.
-    
-  Theorem simu:
-    forall S1 S2,
-      stmt_eval S1 S2 ->
-      forall S1',
-        match_states S1 S1' ->
-        exists S2' t,
-          Smallstep.plus Clight.step1 tge S1' t S2'
-          /\ match_states S2 S2'.
+  Lemma build_co_ok:
+    Ctypes.build_composite_env (map translate_class prog) = Errors.OK (Clight.genv_cenv tge).
   Proof.
-    induction 1;
-    inversion_clear 1 as [? ? ? ? ? ? ? Hvenv Hmenv Hwf Hstmt Hctxt]; 
-    inv Hwf; inversion_clear Hstmt; inversion Hctxt;
-    (((subst s1 || subst s2); inv_stmt_eval) || destruct_conjs).
+    unfold translate in TRANSL.
+    rewrite MAINNODE in TRANSL.
+    unfold Clight.make_program in TRANSL.
+    revert TRANSL.
+    generalize (Clight.make_program_obligation_1
+                  (map translate_class prog)
+                  [(main_id,
+                    make_main
+                      (translate_stmt main_node
+                                      (c_step c_main))
+                      (c_vars c_main))] 
+                  [] main_id).
+    generalize (eq_refl (Ctypes.build_composite_env (map translate_class prog))).
+    intros H1 H2.
+    simpl in H2.
+    admit.
+  Qed.
+  
+  Definition chunk_of_typ ty := AST.chunk_of_type (Ctypes.typ_of_type ty).
+  Definition pointer_of_node node := pointer_of (type_of_inst node).
+  
+  Definition main_fun :=
+    Clight.mkfunction Ctypes.type_int32s AST.cc_default []
+                      c_main.(c_vars)
+                          []
+                          (translate_stmt main_node c_main.(c_step)).
+  
+  Lemma type_pres:
+    forall e, Clight.typeof (translate_exp main_node e) = typeof e.
+  Proof.
+    induction e; simpl; try reflexivity.
+    destruct c; simpl; reflexivity.
+  Qed.
+
+  Definition valid_val (v: val) (t: typ): Prop :=
+    Ctypes.access_mode t = Ctypes.By_value (chunk_of_typ t)
+    /\ v <> Values.Vundef
+    /\ Values.Val.has_type v (Ctypes.typ_of_type t).
+
+  Lemma sem_cast_same:
+    forall v t,
+      valid_val v t ->
+      Cop.sem_cast v t t = Some v.
+  Proof.
+    unfold valid_val; intros; destruct_pairs.
+    destruct t, v;
+      (destruct i, s || destruct f || idtac);
+      (discriminates || contradiction || auto).
+  Qed.
+
+  Inductive well_formed_exp: exp -> Prop :=
+  | wf_var: forall x ty,
+      In (x, ty) c_main.(c_vars) ->
+      x <> self_id ->
+      well_formed_exp (Var x ty)
+  | wf_state: forall x ty,
+      In (x, ty) c_main.(c_mems) ->
+      well_formed_exp (State x ty)
+  | wf_const: forall c ty,
+      well_formed_exp (Const c ty).
+
+  Inductive well_formed_stmt (S: state): stmt -> Prop :=
+  | wf_assign: forall x e v,
+      In (x, typeof e) c_main.(c_vars) ->
+      x <> self_id ->
+      well_formed_exp e ->
+      exp_eval S e v ->
+      valid_val v (typeof e) ->
+      v = Values.Val.load_result (chunk_of_typ (typeof e)) v ->
+      well_formed_stmt S (Assign x e)
+  | wf_assignst: forall x e v,
+      In (x, typeof e) c_main.(c_mems) ->
+      x <> self_id ->
+      well_formed_exp e ->
+      exp_eval S e v ->
+      valid_val v (typeof e) ->
+      v = Values.Val.load_result (chunk_of_typ (typeof e)) v ->
+      well_formed_stmt S (AssignSt x e)
+  | wf_ite: forall e s1 s2,
+      well_formed_exp e ->
+      well_formed_stmt S s1 ->
+      well_formed_stmt S s2 ->
+      well_formed_stmt S (Ifte e s1 s2)
+  | wf_comp: forall S' s1 s2,
+      well_formed_stmt S s1 ->
+      stmt_eval S s1 S' ->
+      well_formed_stmt S' s2 ->
+      well_formed_stmt S (Comp s1 s2)
+  | wf_skip: 
+      well_formed_stmt S Skip.
+
+  Definition compat_venv (S: state) (env: Clight.env) (m: Memory.Mem.mem):  Prop :=
+    forall x v t,
+      find_var x S v ->
+      In (x, t) c_main.(c_vars) ->
+      exists loc,
+        Maps.PTree.get x env = Some (loc, t)
+        /\ Memory.Mem.load (chunk_of_typ t) m loc 0 = Some v
+        /\ valid_val v t.
+
+  Definition compat_menv (S: state) (env: Clight.env) (m: Memory.Mem.mem):  Prop :=
+    forall x v t,
+      find_field x S v ->
+      In (x, t) c_main.(c_mems) ->
+      exists co loc' loc ofs delta,
+        Ctypes.field_offset (Clight.genv_cenv tge) x (Ctypes.co_members co) = Errors.OK delta
+        /\ Memory.Mem.load (chunk_of_typ t) m loc (Int.unsigned (Int.add ofs (Int.repr delta))) = Some v
+        /\ valid_val v t
+        /\ Maps.PTree.get main_node (Clight.genv_cenv tge) = Some co 
+        /\ Maps.PTree.get self_id env = Some (loc', pointer_of_node main_node)
+        /\ Memory.Mem.load (chunk_of_typ (pointer_of_node main_node)) m loc' 0 = Some (Values.Vptr loc ofs)
+        /\ Ctypes.access_mode (pointer_of_node main_node) = Ctypes.By_value (chunk_of_typ (pointer_of_node main_node)).
+
+  Remark valid_val_implies_access:
+    forall v t, valid_val v t -> Ctypes.access_mode t = Ctypes.By_value (chunk_of_typ t).
+  Proof. intros ** H; apply H. Qed.
+    
+  Hint Constructors Clight.eval_lvalue Clight.eval_expr well_formed_stmt.
+  Hint Resolve valid_val_implies_access.
+  
+  Lemma expr_eval_simu:
+    forall S exp v e le m,
+      compat_venv S e m ->
+      compat_menv S e m ->
+      well_formed_exp exp ->
+      exp_eval S exp v ->
+      Clight.eval_expr tge e le m (translate_exp main_node exp) v.
+  Proof.
+    intros S exp;
+    induction exp as [x ty|x ty|c ty];
+    intros ** Hvenv Hmenv Hwf Heval;
+    inv Heval; inv Hwf; simpl.
+
+    (* Var x ty : "x" *)
+    - edestruct Hvenv; destruct_conjs; eauto.
+      eapply Clight.eval_Elvalue, Clight.deref_loc_value; eauto.
+
+    (* State x ty : "self->x" *)
+    - edestruct Hmenv; destruct_conjs; eauto.
+      eapply Clight.eval_Elvalue.
+      + eapply Clight.eval_Efield_struct
+        with (id:=main_node) (att:=Ctypes.noattr); eauto.
+        eapply Clight.eval_Elvalue. 
+        * apply Clight.eval_Ederef. 
+          eapply Clight.eval_Elvalue, Clight.deref_loc_value; eauto.
+        * apply Clight.deref_loc_copy; auto.
+      + eapply Clight.deref_loc_value; eauto.
+
+    (* Const c ty : "c" *)
+    - destruct c; constructor.
+  Qed.
+  
+  Definition compat_vars (e: Clight.env) (m: Memory.Mem.mem): Prop :=
+    forall x t,
+      In (x, t) c_main.(c_vars) ->
+      exists loc,
+        Maps.PTree.get x e = Some (loc, t)
+        /\ Memory.Mem.valid_access m (chunk_of_typ t) loc 0 Memtype.Writable.
+
+  Definition compat_fields (env: Clight.env) (m: Memory.Mem.mem): Prop :=
+    forall x t,
+      In (x, t) c_main.(c_mems) ->
+      exists co loc' loc ofs delta,
+        Ctypes.field_offset (Clight.genv_cenv tge) x (Ctypes.co_members co) = Errors.OK delta
+        /\ In (x, t) (Ctypes.co_members co)
+        /\ Maps.PTree.get main_node (Clight.genv_cenv tge) = Some co
+        /\ Maps.PTree.get self_id env = Some (loc', pointer_of_node main_node)
+        /\ Memory.Mem.load (chunk_of_typ (pointer_of_node main_node)) m loc' 0 = Some (Values.Vptr loc ofs)
+        /\ Memory.Mem.valid_access m (chunk_of_typ t) loc (Int.unsigned (Int.add ofs (Int.repr delta))) Memtype.Writable.
+
+  Definition nodup_env (e: Clight.env) :=
+    forall x x' loc t t',
+      x' <> x ->
+      Maps.PTree.get x e = Some (loc, t) ->
+      Maps.PTree.get x' e <> Some (loc, t').
+
+  Definition nodup_fields (co: Ctypes.composite) :=
+    forall x t t',
+      In (x, t) (Ctypes.co_members co) ->
+      In (x, t') (Ctypes.co_members co) ->
+      t' = t.
+
+  Definition nodup_vars :=
+    forall x t t',
+      In (x, t) c_main.(c_vars) ->
+      In (x, t') c_main.(c_vars) ->
+      t' = t.
+
+   Definition nodup_mems :=
+    forall x t t',
+      In (x, t) c_main.(c_mems) ->
+      In (x, t') c_main.(c_mems) ->
+      t' = t.
+  
+  Remark find_add:
+    forall x (v v': val) pm, 
+      PM.find x (PM.add x v pm) = Some v' -> v' = v.
+  Proof.
+    induction x, pm; simpl; (eauto || now injection 1).
+  Qed.
+
+  Remark find_update_var:
+    forall x v v' S,
+      find_var x (update_var x S v) v' -> v' = v.
+  Proof.
+    unfold find_var, update_var; simpl.
+    intros; eapply find_add; eauto.
+  Qed.
+
+  Remark find_update_field:
+    forall x v v' S,
+      find_field x (update_field x S v) v' -> v' = v.
+  Proof.
+    unfold find_field, update_field, mfind_mem, madd_mem; simpl.
+    intros; eapply find_add; eauto.
+  Qed.
+
+  Remark gso_var:
+    forall x x' v v' S,
+      x <> x' -> find_var x (update_var x' S v) v' -> find_var x S v'.
+  Proof.
+    unfold find_var, update_var; simpl.
+    intros ** Neq H.
+    rewrite <-H; symmetry.
+    apply PM.gso; auto.
+  Qed.
+
+  Remark gso_field:
+    forall x x' v v' S,
+      x <> x' -> find_field x (update_field x' S v) v' -> find_field x S v'.
+  Proof.
+    unfold find_field, update_field; simpl.
+    intros ** Neq H.
+    rewrite <-H; symmetry.
+    apply mfind_mem_gso; auto.
+  Qed.
+  
+  Definition mem_sep (e: Clight.env) (m: Memory.Mem.mem) :=
+    forall x loc t (* co x' *) ofs (* delta t' *) loc' (* v *) loc'',
+      In (x, t) c_main.(c_vars) -> 
+      Maps.PTree.get x e = Some (loc, t) ->
+      Maps.PTree.get self_id e = Some (loc'', pointer_of_node main_node) ->
+      (* Maps.PTree.get main_node (Clight.genv_cenv tge) = Some co -> *)
+      (* Ctypes.field_offset (Clight.genv_cenv tge) x' (Ctypes.co_members co) = Errors.OK delta -> *)
+      (* Memory.Mem.load (chunk_of_typ t') m loc' (Int.unsigned (Int.add ofs (Int.repr delta))) = Some v -> *)
+      Memory.Mem.load (chunk_of_typ (pointer_of_node main_node)) m loc'' 0 = Some (Values.Vptr loc' ofs) ->
+      loc <> loc'.
+
+  Definition self_sep (e: Clight.env) (m: Memory.Mem.mem) :=
+    forall loc ofs loc',
+      Maps.PTree.get self_id e = Some (loc', pointer_of_node main_node) ->
+      Memory.Mem.load (chunk_of_typ (pointer_of_node main_node)) m loc' 0 = Some (Values.Vptr loc ofs) ->
+      loc <> loc'.
+
+  Definition fields_sep (m: Memory.Mem.mem) :=
+    forall co x x' t t' ofs delta delta',
+      x <> x' ->
+      Ctypes.field_offset (Clight.genv_cenv tge) x (Ctypes.co_members co) = Errors.OK delta ->
+      Ctypes.field_offset (Clight.genv_cenv tge) x' (Ctypes.co_members co) = Errors.OK delta' ->
+      (BinInt.Z.le
+         (BinInt.Z.add (Int.unsigned (Int.add ofs (Int.repr delta')))
+                       (Memdata.size_chunk (chunk_of_typ t')))
+         (Int.unsigned (Int.add ofs (Int.repr delta)))
+       \/
+       BinInt.Z.le
+         (BinInt.Z.add (Int.unsigned (Int.add ofs (Int.repr delta)))
+                       (Memdata.size_chunk (chunk_of_typ t)))
+         (Int.unsigned (Int.add ofs (Int.repr delta')))).
+      
+  
+  Ltac clear_refl_trivial :=
+    match goal with
+    | H: ?x = ?x |- _ => clear H
+    end.
+  Ltac clear_refl_trivials := repeat clear_refl_trivial.
+  Ltac clean_context := clear_dups; clear_refl_trivials.
+  
+  Lemma compat_assign_pres:
+    forall S env m loc x e v,
+      compat_venv S env m ->
+      compat_menv S env m ->
+      compat_vars env m ->
+      compat_fields env m ->
+      mem_sep env m ->
+      self_sep env m ->
+      nodup_env env ->
+      nodup_vars ->
+      Maps.PTree.get x env = Some (loc, typeof e) ->
+      In (x, typeof e) c_main.(c_vars) ->
+      v = Values.Val.load_result (chunk_of_typ (typeof e)) v ->
+      valid_val v (typeof e) ->
+      x <> self_id ->
+      Memory.Mem.valid_access m (chunk_of_typ (typeof e)) loc 0 Memtype.Writable ->
+      exp_eval S e v ->
+      exists m', Memory.Mem.store (chunk_of_typ (typeof e)) m loc 0 v = Some m' 
+            /\ compat_venv (update_var x S v) env m'
+            /\ compat_menv S env m'
+            /\ compat_vars env m' 
+            /\ compat_fields env m' 
+            /\ mem_sep env m'
+            /\ self_sep env m'.
+  Proof.
+    intros ** Hvenv Hmenv Hvars Hfields Hsep Hself_sep Hnodupenv Hnodupvars Hget Hin Hloadres ? ? ? ?.
+    edestruct Memory.Mem.valid_access_store with (v:=v) as [m']; eauto. 
+    exists m'; repeat split; auto; clean_context.
+    - unfold compat_venv; intros x' v' t' Hfind Hin'.
+      destruct (AST.ident_eq x' x) as [|Hx].
+      + subst x'.
+        apply find_update_var in Hfind; subst v'.
+        generalize (Hnodupvars _ _ _ Hin Hin'); intro; subst t'. 
+        exists loc; split; [|split]; auto.
+        rewrite Hloadres; eapply Memory.Mem.load_store_same; eauto.
+      + apply gso_var in Hfind; auto.
+        edestruct Hvenv as [loc' [? [Hload]]]; eauto.
+        exists loc'; split; [|split]; auto. 
+        destruct (Values.eq_block loc' loc).
+        * subst loc'.
+          edestruct Hnodupenv; eauto. 
+        * rewrite <-Hload. 
+          eapply Memory.Mem.load_store_other; eauto.
+    - unfold compat_menv; intros x' v' t' Hmem Hin'.
+      edestruct Hmenv
+        as (co & loc'' & loc' & ofs & delta & ? & Hload & ? & ? & Hself' & Hloadptr & ?); eauto.
+      exists co, loc'', loc', ofs, delta.
+      split; [|split; [|split; [|repeat split]]]; auto.
+      + destruct (Values.eq_block loc loc').
+        * edestruct Hsep with (2:=Hget); eauto; contradiction.
+        * rewrite <-Hload.
+          eapply Memory.Mem.load_store_other; eauto.
+      + destruct (Values.eq_block loc'' loc).
+        * subst loc''.
+          edestruct Hnodupenv with (2:=Hget); eauto.
+        * rewrite <-Hloadptr.
+          eapply Memory.Mem.load_store_other; eauto.
+    - unfold compat_vars; intros x' t' Hin'.
+      edestruct Hvars as (loc' & ? & ?); eauto.
+      exists loc'; split; auto.
+      eapply Memory.Mem.store_valid_access_1; eauto.
+    - unfold compat_fields; intros x' t' Hin'.
+      edestruct Hfields as (co & loc1' & loc1 & ofs & delta & ? & ? & ? & ? & Hload & ?); eauto. 
+      exists co, loc1', loc1, ofs, delta; split; [|split; [|split; [|split; [|split]]]]; auto.
+      + destruct (Values.eq_block loc1' loc).
+        * subst loc1'.
+          edestruct Hnodupenv with (2:=Hget); eauto.
+        * rewrite <-Hload; eapply Memory.Mem.load_store_other; eauto.
+      + eapply Memory.Mem.store_valid_access_1; eauto.
+    - unfold mem_sep; intros x' loc1 t' ofs loc1' loc1'' Hin1 Hget1 Hself Hload.
+      eapply Hsep; eauto.
+      instantiate (1:=ofs).
+      destruct (Values.eq_block loc1'' loc).
+      + subst loc1''.
+        edestruct Hnodupenv with (2:=Hget); eauto.
+      + rewrite <-Hload; symmetry; eapply Memory.Mem.load_store_other; eauto.
+    - unfold self_sep; intros loc1 ofs loc1' Hself Hload.
+      eapply Hself_sep; eauto.
+      instantiate (1:=ofs).
+      destruct (Values.eq_block loc1' loc).
+      + subst loc1'.
+        edestruct Hnodupenv with (2:=Hget); eauto.
+      + rewrite <-Hload; symmetry; eapply Memory.Mem.load_store_other; eauto.
+  Qed.
+
+   Lemma compat_stassign_pres:
+    forall S env m x e v co loc loc' ofs delta,
+      compat_venv S env m ->
+      compat_menv S env m ->
+      compat_vars env m ->
+      compat_fields env m ->
+      mem_sep env m ->
+      self_sep env m ->
+      fields_sep m ->
+      nodup_mems ->
+      In (x, (typeof e)) (Ctypes.co_members co) ->
+      Ctypes.field_offset tge.(Clight.genv_cenv) x (Ctypes.co_members co) = Errors.OK delta ->
+      Maps.PTree.get main_node (Clight.genv_cenv tge) = Some co ->
+      Maps.PTree.get self_id env = Some (loc', pointer_of_node main_node) ->
+      Memory.Mem.load (chunk_of_typ (pointer_of_node main_node)) m loc' 0 = Some (Values.Vptr loc ofs) ->
+      In (x, typeof e) c_main.(c_mems) ->
+      v = Values.Val.load_result (chunk_of_typ (typeof e)) v ->
+      valid_val v (typeof e) ->
+     Memory.Mem.valid_access m (chunk_of_typ (typeof e)) loc (Int.unsigned (Int.add ofs (Int.repr delta))) Memtype.Writable ->
+      exp_eval S e v ->
+      exists m',
+        Memory.Mem.store (chunk_of_typ (typeof e)) m loc (Int.unsigned (Int.add ofs (Int.repr delta))) v = Some m'
+        /\ compat_venv S env m'
+        /\ compat_menv (update_field x S v) env m'
+        /\ compat_vars env m'
+        /\ compat_fields env m'
+        /\ mem_sep env m'
+        /\ self_sep env m'.
+  Proof.
+    intros ** Hvenv Hmenv Hvars Hfields Hsep Hself_sep Hfields_sep Hnodupmems Hmembers Hoffset Hmain Hself Hloadptr Hin Hloadres ? ? ?.
+    edestruct Memory.Mem.valid_access_store with (v:=v) as [m']; eauto. 
+    exists m'; repeat (split; auto); clean_context.
+    - unfold compat_venv; intros x' v' t' Hmto Hin'.
+      edestruct Hvenv as (loc'' & Hget & Hload' & ?); eauto.
+      exists loc''; split; [|split]; auto.
+      destruct (Values.eq_block loc'' loc).
+      + edestruct Hsep with (1:=Hin'); eauto.
+      + rewrite <-Hload'.
+        eapply Memory.Mem.load_store_other; eauto.
+    - unfold compat_menv; intros x' v' t' Hmem Hin'.
+      destruct (AST.ident_eq x' x).
+      + subst x'.
+        apply find_update_field in Hmem; subst v'.
+        generalize (Hnodupmems _ _ _ Hin Hin'); intro; subst t'. 
+        exists co, loc', loc, ofs, delta.
+        split; [|split; [|split; [|split; [|repeat split]]]]; auto.
+        * rewrite Hloadres; eapply Memory.Mem.load_store_same; eauto.
+        *{ destruct (Values.eq_block loc' loc).
+           - edestruct Hself_sep; eauto.  
+           - rewrite <-Hloadptr.
+             eapply Memory.Mem.load_store_other; eauto.
+         }
+      + apply gso_field in Hmem; auto.
+        edestruct Hmenv
+          as (co' & loc1' & loc1 & ofs' & delta' & ? & Hload' & ? & Hmain1 & Hself1 & Hloadptr1 & ?); eauto. 
+        rewrite Hmain in Hmain1; inversion Hmain1; subst co'.
+        rewrite Hself in Hself1; inversion Hself1; subst loc1'.
+        rewrite Hloadptr in Hloadptr1; inversion Hloadptr1; subst loc1 ofs'.
+        exists co, loc', loc, ofs, delta'.
+        split; [|split; [|split; [|split; [|repeat split]]]]; auto.
+        * rewrite <-Hload'. eapply Memory.Mem.load_store_other; eauto. 
+        *{ destruct (Values.eq_block loc' loc).
+           - edestruct Hself_sep; eauto. 
+           - rewrite <-Hloadptr.
+             eapply Memory.Mem.load_store_other; eauto.
+         }
+    - unfold compat_vars; intros x' t' Hin'.
+      edestruct Hvars as (loc1' & ? & ?); eauto.
+      exists loc1'; split; auto.
+      eapply Memory.Mem.store_valid_access_1; eauto.
+    - unfold compat_fields; intros x' t' Hin'.
+      edestruct Hfields as (co' & loc1' & loc1 & ofs' & delta' & ? & ? & ? & Hself' & Hload & ?); eauto. 
+      exists co', loc1', loc1, ofs', delta'; split; [|split; [|split; [|split; [|split]]]]; auto.
+      + destruct (Values.eq_block loc1' loc).
+        * subst loc1'.
+          rewrite Hself in Hself'; inversion Hself'. subst loc'.
+          edestruct Hself_sep; eauto.
+        * rewrite <-Hload; eapply Memory.Mem.load_store_other; eauto.
+      + eapply Memory.Mem.store_valid_access_1; eauto.          
+    - unfold mem_sep; intros x' loc1 t' ofs' loc1' loc1'' Hin1 Hget1 Hself' Hload.
+      eapply Hsep; eauto.
+      instantiate (1:=ofs').
+      destruct (Values.eq_block loc1'' loc).
+      + subst loc1''.
+        rewrite Hself in Hself'; inversion Hself'. subst loc'.
+        edestruct Hself_sep; eauto.  
+      + rewrite <-Hload; symmetry; eapply Memory.Mem.load_store_other; eauto.
+    - unfold self_sep; intros loc1 ofs' loc1' Hself' Hload.
+      eapply Hself_sep; eauto.
+      instantiate (1:=ofs').
+      destruct (Values.eq_block loc1' loc).
+      + subst loc1'.
+        rewrite Hself in Hself'; inversion Hself'. subst loc'.
+        edestruct Hself_sep; eauto.  
+      + rewrite <-Hload; symmetry; eapply Memory.Mem.load_store_other; eauto.
+  Qed.
+
+Remark ifte_translate:
+    forall (b: bool) s1 s2,
+      translate_stmt main_node (if b then s1 else s2) =
+      if b then (translate_stmt main_node s1) else (translate_stmt main_node s2).
+  Proof.
+    now destruct b.
+  Qed.  
+
+  Hint Constructors Clight.eval_lvalue Clight.eval_expr well_formed_stmt.
+  Hint Resolve expr_eval_simu Clight.assign_loc_value sem_cast_same.
+  Hint Constructors well_formed_stmt.
+
+  Definition c_state := (Clight.env * Clight.temp_env * Memory.Mem.mem)%type.
+   
+  Inductive match_states_bigbig (S: state): c_state -> Prop :=
+    intro_state_bigbig: forall e le m,
+      (* state correspondance *)
+      compat_venv S e m ->     
+      compat_menv S e m ->
+      
+      (* Clight state well defined *)
+      compat_vars e m ->
+      compat_fields e m ->
+
+      (* Clight side separation *)
+      mem_sep e m ->
+      self_sep e m ->
+      fields_sep m ->
+      nodup_env e ->
+
+      (* Minimp side separation *)
+      nodup_vars ->
+      nodup_mems ->
+      match_states_bigbig S (e, le, m).
+
+  Hint Constructors match_states_bigbig.
+
+  Theorem simu_bigbig:
+    forall S1 s S2,
+      well_formed_stmt S1 s ->
+      stmt_eval S1 s S2 ->
+      forall e1 le1 m1,
+        match_states_bigbig S1 (e1, le1, m1) ->
+        exists le2 m2 t,
+          ClightBigstep.exec_stmt tge e1 le1 m1 (translate_stmt main_node s) t le2 m2 ClightBigstep.Out_normal
+          /\ match_states_bigbig S2 (e1, le2, m2).
+  Proof.
+    induction 2; inversion_clear H; 
+    inversion_clear 1 as [? ? ? Hvenv Hmenv Hvars Hfields].
     
     (* Assign x e : "x = e" *)
     - app_exp_eval_det.
-      edestruct compat_assign_pres as [m']; eauto; destruct_conjs. 
-      do 2 econstructor; split.
-      + eapply Smallstep.plus_one, Clight.step_assign; eauto.
-        * eapply expr_eval_simu; eauto.
-        * rewrite type_pres; auto. 
+      edestruct Hvars; eauto.
+      edestruct compat_assign_pres as [m']; destruct_conjs; eauto.
+      do 3 econstructor; split.
+      + eapply ClightBigstep.exec_Sassign; eauto. 
+        rewrite type_pres; auto. 
       + constructor; auto. 
-        
+
     (* AssignSt x e : "self->x = e"*)
     - app_exp_eval_det.
-      edestruct compat_stassign_pres as [m']; eauto; destruct_conjs.
-      do 2 econstructor; split.
-      + eapply Smallstep.plus_one, Clight.step_assign; eauto.
+      edestruct Hfields; eauto; destruct_conjs.
+      edestruct compat_stassign_pres as [m']; eauto; destruct_conjs. 
+      do 3 econstructor; split.
+      + eapply ClightBigstep.exec_Sassign; eauto.
         *{ eapply Clight.eval_Efield_struct
            with (id:=main_node) (att:=Ctypes.noattr); eauto.
            eapply Clight.eval_Elvalue; eauto. 
@@ -120,54 +564,25 @@ Section SIMU.
              apply Clight.deref_loc_value with (chunk:=AST.Mint32); eauto.
            - apply Clight.deref_loc_copy; auto.
          }
-        * eapply expr_eval_simu; eauto.
         * rewrite type_pres; auto. 
-      + constructor; auto.
+      + constructor; auto. 
 
     (* Ifte e s1 s2 : "if e then s1 else s2" *)
-    - app_exp_eval_det.
-      pose proof (bool_val_ptr v _ m0 m H0) as Hptr.
-      rewrite Hptr in H24. rewrite H1 in H24; inversion H24; subst b0; clear H24.
-      edestruct IHstmt_eval as [S2' [t1 [Step1 ?]]]; eauto.
-      do 2 econstructor; split; eauto.
-      eapply Smallstep.plus_left'; eauto.
-      rewrite ifte_translate.
-      eapply Clight.step_ifthenelse.
-      + eapply expr_eval_simu; eauto.
-      + erewrite type_pres, bool_val_ptr; eauto.  
-      
-    (* Comp s1 s2 : "s1; s2" *)
-    - repeat app_stmt_eval_det.
-      edestruct IHstmt_eval1 as [S2' [t1 [Step1 ?]]]; eauto.
-      edestruct IHstmt_eval2 as [S3' [t2 [Step2 ?]]]; eauto.
-      do 2 econstructor; split; eauto.
-      eapply Smallstep.plus_left' with
-      (s2:=Clight.State (main_fun main_node c_main) (translate_stmt main_node s1)
-                        (Clight.Kseq (translate_stmt main_node s2) k) e le m)
-        (t1:=Events.E0) (t2:=Events.E0); auto.
-      + eapply Clight.step_seq.
-      + eapply Smallstep.plus_trans; eauto.
-        *{ eapply Smallstep.plus_left' with
-          (s2:=Clight.State (main_fun main_node c_main) (translate_stmt main_node s2) k e le m')
-            (t1:=Events.E0) (t2:=Events.E0); auto.
-           - assert (S2' = Clight.State (main_fun main_node c_main)
-                                        (translate_stmt main_node Skip)
-                                        (Clight.Kseq (translate_stmt main_node s2) k) e le m'). admit. subst S2'.
-             apply Clight.step_skip_seq.
-           - assert (t2 = Events.E0). admit. subst t2; auto.
-         }
-        * assert (t1 = Events.E0). admit. subst t1; auto.
+    - edestruct IHstmt_eval as (le2 & m2 & t & ? & ?); eauto;
+      [destruct b|]; auto.
+      do 3 econstructor; split; eauto.
+      eapply ClightBigstep.exec_Sifthenelse; eauto.
+      + erewrite type_pres, bool_val_ptr; eauto. 
+      + fold translate_stmt; rewrite <-ifte_translate; eauto.
 
-    (* Comp Skip s : "skip; s" *)
-    - repeat app_stmt_eval_det.
-      edestruct IHstmt_eval as [S2' [t1 [Step1 Match2]]]; eauto.
-      do 2 econstructor; split; eauto.
-      eapply Smallstep.plus_left' with
-      (s2:=Clight.State (main_fun main_node c_main) (translate_stmt main_node Skip)
-                        (Clight.Kseq (translate_stmt main_node s) k) e le m)
-        (t1:=Events.E0) (t2:=Events.E0); eauto.
-      + eapply Clight.step_seq.
-      + eapply Smallstep.plus_left'; eauto.
-        * apply Clight.step_skip_seq.
-        * assert (t1 = Events.E0). admit. subst t1; auto.
+    (* Comp s1 s2 : "s1; s2" *)
+    - app_stmt_eval_det.
+      edestruct IHstmt_eval1 as (le2 & m2 & t1 & ? & ?); eauto.
+      edestruct IHstmt_eval2 as (le3 & m3 & t2 & ? & ?); eauto.
+      do 3 econstructor; split; eauto.
+      eapply ClightBigstep.exec_Sseq_1; eauto.
+     
+    (* Skip : "skip" *)
+    - do 3 econstructor; split; eauto.
+      eapply ClightBigstep.exec_Sskip.
   Qed.
