Simu/Sem.v
@@ -1,78 +1,279 @@
-Require Import CommonSem.
+Require common.Values cfrontend.Cop.
+Require Import lib.Integers lib.Floats.
+        
+Require Export Rustre.Common.
+Require Export Rustre.RMemory.
 
-Definition state := (menv * venv * stmt)%type.
+Require Export Syn.
 
-(* =stmt_eval= *)
-Inductive stmt_eval: state -> state -> Prop :=
-| Iassign: forall me ve x e v ve',
-    exp_eval me ve e v ->
-    PM.add x v ve = ve' ->
-    stmt_eval (me, ve, Assign x e) (me, ve', Skip)
-| Iassignst: forall me ve x e v me',
-    exp_eval me ve e v ->
-    madd_mem x v me = me' ->
-    stmt_eval (me, ve, AssignSt x e) (me', ve, Skip)
-| Iifte: forall me ve m e v b s1 s2 me' ve',
-    exp_eval me ve e v ->
-    (forall ty attr, Ctypes.typeconv (typeof e) <> Ctypes.Tpointer ty attr) ->
-    Cop.bool_val v (typeof e) m = Some b ->
-    stmt_eval (me, ve, if b then s1 else s2) (me', ve', Skip) ->
-    stmt_eval (me, ve, Ifte e s1 s2) (me', ve', Skip)
-| Icomp: forall me1 ve1 s1 me2 ve2 s2 me3 ve3,
-    stmt_eval (me1, ve1, s1) (me2, ve2, Skip) ->
-    stmt_eval (me2, ve2, s2) (me3, ve3, Skip) ->
-    stmt_eval (me1, ve1, Comp s1 s2) (me3, ve3, Skip)
-| Iskip_comp: forall me ve s me' ve',
-    stmt_eval (me, ve, s) (me', ve', Skip) ->
-    stmt_eval (me, ve, Comp Skip s) (me', ve', Skip)
-(* | Icomp_skip: forall me ve s me' ve', *)
-(*     stmt_eval (me, ve, s) (me', ve', Skip) -> *)
-(*     stmt_eval (me, ve, Comp s Skip) (me', ve', Skip) *).
-(** ** Determinism of semantics *)
+Ltac inv H := inversion H; clear H; subst.
+
+(* SEMANTICS *)
+Definition val: Type := Values.val.
+
+Definition menv: Type := memory val.
+Definition venv: Type := PM.t val.
+
+Definition m_empty: menv := empty_memory _.
+Definition v_empty: venv := PM.empty val.
+
+Definition state := (menv * venv)%type.
+
+Definition find_var (x: ident) (S: state) (v: val) := PM.find x (snd S) = Some v.
+Definition find_field (x: ident) (S: state) (v: val) := mfind_mem x (fst S) = Some v.
+
+Definition val_of_const c :=
+  match c with
+  | Cint i => Values.Vint i
+  | Cfloat f => Values.Vfloat f
+  | Csingle s => Values.Vsingle s
+  | Clong l => Values.Vlong l
+  end.
+
+Lemma bool_val_ptr:
+  forall v t m m',
+    (forall ty attr, Ctypes.typeconv t <> Ctypes.Tpointer ty attr) ->
+    Cop.bool_val v t m = Cop.bool_val v t m'.
+Proof.
+  intros.
+  unfold Cop.bool_val.
+  destruct v, t; try destruct i0; try destruct f; simpl in *;
+  (auto || (edestruct H; eauto)). 
+Qed.
+
+Inductive exp_eval (S: state): exp -> val -> Prop :=
+| evar: forall x v ty,
+    find_var x S v ->
+    exp_eval S (Var x ty) v
+| estate: forall x v ty,
+    find_field x S v ->
+    exp_eval S (State x ty) v
+| econst: forall c ty,
+    exp_eval S (Const c ty) (val_of_const c).
+
+Remark find_var_det:
+  forall x v1 v2 S,
+    find_var x S v1 ->
+    find_var x S v2 ->
+    v1 = v2.
+Proof.
+  unfold find_var.
+  intros ** H1 H2.
+  rewrite H1 in H2; inv H2; reflexivity.
+Qed.
+
+Remark find_field_det:
+  forall x v1 v2 S,
+    find_field x S v1 ->
+    find_field x S v2 ->
+    v1 = v2.
+Proof.
+  unfold find_field.
+  intros ** H1 H2.
+  rewrite H1 in H2; inv H2; reflexivity.
+Qed.
 
 Theorem exp_eval_det:
-  forall me ve e v1 v2,
-    exp_eval me ve e v1 ->
-    exp_eval me ve e v2 ->
+  forall S e v1 v2,
+    exp_eval S e v1 ->
+    exp_eval S e v2 ->
     v1 = v2.
 Proof.
   induction e; intros v1 v2 H1 H2;
   inversion H1 as [? ? ? Hv1|? ? ? Hv1|];
   inversion H2 as [? ? ? Hv2|? ? ? Hv2|];
-  auto; unfold PM.MapsTo in *; rewrite Hv1 in Hv2; now injection Hv2.
+  [eapply find_var_det; eauto|eapply find_field_det; eauto|auto]. 
 Qed.
 
 Ltac app_exp_eval_det :=
   match goal with
-  | H1: exp_eval ?me ?ve ?e ?v1,
-        H2: exp_eval ?me ?ve ?e ?v2 |- _ =>
+  | H1: exp_eval ?S ?e ?v1,
+        H2: exp_eval ?S ?e ?v2 |- _ =>
     assert (v1 = v2) by (eapply exp_eval_det; eauto); subst v2; clear H2 
   end.
 
-Ltac inv_stmt_eval :=
+Definition update_var (x: ident) (S: state) (v: val) := (fst S, PM.add x v (snd S)).
+Definition update_field (x: ident) (S: state) (v: val) := (madd_mem x v (fst S), snd S).
+
+(* =stmt_eval= *)
+Inductive stmt_eval (S: state): stmt -> state -> Prop :=
+| Iassign: forall x e v,
+    exp_eval S e v ->
+    stmt_eval S (Assign x e) (update_var x S v)
+| Iassignst: forall x e v,
+    exp_eval S e v ->
+    stmt_eval S (AssignSt x e) (update_field x S v)
+| Iifte: forall e m v b s1 s2 S',
+    exp_eval S e v ->
+    (forall ty attr, Ctypes.typeconv (typeof e) <> Ctypes.Tpointer ty attr) ->
+    Cop.bool_val v (typeof e) m = Some b ->
+    stmt_eval S (if b then s1 else s2) S' ->
+    stmt_eval S (Ifte e s1 s2) S'    
+| Icomp: forall s1 S2 s2 S3,
+    stmt_eval S s1 S2 ->
+    stmt_eval S2 s2 S3 ->
+    stmt_eval S (Comp s1 s2) S3
+| Iskip: 
+    stmt_eval S Skip S.
+
+Ltac app_bool_val :=
   match goal with
-  | H: stmt_eval (_, _, Skip) _ |- _ => inversion H
-  end.
+  | H: forall ty attr, Ctypes.typeconv ?t <> Ctypes.Tpointer ty attr,
+    H1: Cop.bool_val ?v ?t ?m = Some ?b,
+    H2: Cop.bool_val ?v ?t ?m' = Some ?b' |- _ =>
+let Heq := fresh in
+pose proof (bool_val_ptr v _ m m' H) as Heq; rewrite Heq in H1; rewrite H1 in H2; inv H2
+end.
 
 Theorem stmt_eval_det:
-  forall st st1 st2,
-    stmt_eval st st1 ->
-    stmt_eval st st2 ->
-    st1 = st2.
+  forall S s S1 S2,
+    stmt_eval S s S1 ->
+    stmt_eval S s S2 ->
+    S1 = S2.
 Proof.
-  intros.
-  revert st2 H0. induction H; intros st2 H2'; inv H2';
-                 ((app_exp_eval_det; auto) || inv_stmt_eval || idtac).
-  - pose proof (bool_val_ptr v _ m0 m H0) as Hptr. rewrite Hptr in H11. rewrite H1 in H11; inv H11. apply IHstmt_eval in H12; auto.
-  - apply IHstmt_eval1 in H6. inv H6. apply IHstmt_eval2; auto.
-  - apply IHstmt_eval in H4; auto.
-  (* - apply IHstmt_eval in H5; auto. *)
+  intros until S2; intro Hev1; revert S2;
+  induction Hev1; intros S2' Hev2; inv Hev2;
+  try app_exp_eval_det; auto.
+  - apply IHHev1.
+    app_bool_val; auto.
+  - assert (S2 = S0) as Heq by now apply IHHev1_1.
+    apply IHHev1_2; rewrite Heq; auto.
 Qed.
 
 Ltac app_stmt_eval_det :=
   match goal with
-  | H1: stmt_eval ?st (?me1, ?ve1, ?s1),
-        H2: stmt_eval ?st (?me2, ?ve2, ?s2) |- _ =>
+  | H1: stmt_eval ?S ?s ?S1,
+        H2: stmt_eval ?S ?s ?S2 |- _ =>
     let H := fresh in
-    assert ((me2, ve2, s2) = (me1, ve1, s1)) as H by (eapply stmt_eval_det; eauto); inv H; clear H2
+    assert (S2 = S1) as H by (eapply stmt_eval_det; eauto); inv H; clear H2
   end.
+
+(* Inductive cont := *)
+(* | Kstop: cont *)
+(* | Kseq: stmt -> cont -> cont. *)
+
+(* (* =stmt_eval= *) *)
+(* Inductive stmt_eval_cont: state * stmt * cont -> state * stmt * cont -> Prop := *)
+(* | Iassign_cont: forall me ve x e v ve' k, *)
+(*     exp_eval me ve e v -> *)
+(*     PM.add x v ve = ve' -> *)
+(*     stmt_eval_cont ((me, ve), Assign x e, k) ((me, ve'), Skip, k) *)
+(* | Iassignst_cont: forall me ve x e v me' k, *)
+(*     exp_eval me ve e v -> *)
+(*     madd_mem x v me = me' -> *)
+(*     stmt_eval_cont ((me, ve), AssignSt x e, k) ((me', ve), Skip, k) *)
+(* | Iifte_cont: forall me ve m e v b s1 s2 k, *)
+(*     exp_eval me ve e v -> *)
+(*     (forall ty attr, Ctypes.typeconv (typeof e) <> Ctypes.Tpointer ty attr) -> *)
+(*     Cop.bool_val v (typeof e) m = Some b -> *)
+(*     stmt_eval_cont ((me, ve), Ifte e s1 s2, k) ((me, ve), if b then s1 else s2, k)     *)
+(* | Icomp_cont: forall st s1 s2 k, *)
+(*     stmt_eval_cont (st, Comp s1 s2, k) (st, s1, Kseq s2 k) *)
+(* | Iskip_comp_cont: forall st s k, *)
+(*     stmt_eval_cont (st, Skip, Kseq s k) (st, s, k). *)
+
+(* Section SEQUENCES. *)
+(*   Set Implicit Arguments. *)
+
+(*   Variable A: Type.  *)
+(*   Variable R: A -> A -> Prop.  *)
+
+(*   Inductive star: A -> A -> Prop := *)
+(*   | star_refl: forall a, *)
+(*       star a a *)
+(*   | star_step: forall a b c, *)
+(*       R a b -> star b c -> star a c. *)
+
+(*   Hint Constructors star. *)
+
+(*   Lemma star_one: *)
+(*     forall (a b: A), R a b -> star a b. *)
+(*   Proof. *)
+(*     intros. econstructor; eauto.  *)
+(*   Qed. *)
+
+(*   Lemma star_trans: *)
+(*     forall (a b: A), star a b -> forall c, star b c -> star a c. *)
+(*   Proof. *)
+(*     induction 1; intros. auto. econstructor; eauto. *)
+(*   Qed. *)
+
+(*   Lemma one_star_trans: *)
+(*     forall (a b: A), R a b -> forall c, star b c -> star a c. *)
+(*   Proof. *)
+(*     intros. econstructor; eauto. *)
+(*   Qed. *)
+
+(* End SEQUENCES. *)
+
+(* Definition terminates (S: state) (s: stmt) (S': state) : Prop := *)
+(*   star stmt_eval_cont (S, s, Kstop) (S', Skip, Kstop). *)
+
+(* Hint Resolve star_one star_trans one_star_trans.  *)
+(* Hint Constructors star stmt_eval_cont. *)
+
+(* Theorem to_cont: *)
+(*   forall S s S', *)
+(*     stmt_eval S s S' -> *)
+(*     forall k, star stmt_eval_cont (S, s, k) (S', Skip, k). *)
+(* Proof. *)
+(*   induction 1; eauto. *)
+(* Qed. *)
+
+
+(* Inductive keval: cont -> state -> state -> Prop := *)
+(* | KE_stop: forall S, *)
+(*     keval Kstop S S *)
+(* | KE_seq: forall s k S S' S'', *)
+(*     stmt_eval S s S' -> *)
+(*     keval k S' S'' -> *)
+(*     keval (Kseq s k) S S''. *)
+
+(* Inductive skeval: state * stmt * cont -> state -> Prop := *)
+(*   ske_intro: forall s k S S' S'', *)
+(*       stmt_eval S s S' -> *)
+(*       keval k S' S'' -> *)
+(*       skeval (S, s, k) S''. *)
+
+(* Require Import Coq.Program.Equality. *)
+
+(* Hint Constructors stmt_eval. *)
+
+(* Lemma stmt_eval_cont_skeval: *)
+(*   forall S s k S' s' k', *)
+(*     stmt_eval_cont (S, s, k) (S', s', k') -> *)
+(*     forall S'', *)
+(*       skeval (S', s', k') S'' -> *)
+(*       skeval (S, s, k) S''. *)
+(* Proof. *)
+(*   intros until k'. intro STEP. dependent induction STEP; intros. *)
+(*   - inv H0. inv H5. econstructor; eauto; auto. *)
+(*   - inv H0. inv H5. econstructor; eauto; auto. *)
+(*   - inv H2. destruct S'. econstructor. econstructor; eauto. auto. *)
+(*   - inv H. inv H5. econstructor; eauto. destruct S', S'1, S'0. econstructor; eauto. *)
+(*   - inv H. econstructor; eauto. econstructor; eauto. *)
+(* Qed. *)
+
+(* Lemma stmt_eval_cont_skeval': *)
+(*   forall S s k S' s' k' S'', *)
+(*     star stmt_eval_cont (S, s, k) (S', s', k') -> *)
+(*     skeval (S', s', k') S'' -> *)
+(*     skeval (S, s, k) S''. *)
+(* Proof. *)
+(*   intros; dependent induction H; auto. *)
+(*   destruct b as [[S1 s1] k1]. *)
+(*   eapply stmt_eval_cont_skeval; eauto. *)
+(* Qed. *)
+
+(* Hint Constructors keval. *)
+
+(* Theorem from_cont: *)
+(*   forall S s S', *)
+(*   terminates S s S' -> stmt_eval S s S'. *)
+(* Proof. *)
+(*   unfold terminates; intros. *)
+(*   assert (SKEV: skeval (S, s, Kstop) S'). *)
+(*   - eapply stmt_eval_cont_skeval'; eauto. *)
+(*     econstructor; eauto.  *)
+(*   - inv SKEV. inv H5; auto. *)
+(* Qed. *)
